feat: make labels extensional

src/core/DY.Core.Label.fst
@@ -4,6 +4,8 @@ open DY.Core.Label.Type
 open DY.Core.Trace.Type
 open DY.Core.Trace.Base
 
+#set-options "--fuel 0 --ifuel 0"
+
 /// This module define the notion of corruption of a label (`is_corrupt`),
 /// and the flow relation between labels (`can_flow`),
 /// along with theorems that can be used to reason on the label flow.
@@ -35,6 +37,53 @@ open DY.Core.Trace.Base
 /// This notion of "less secret" is lifted to labels,
 /// using the flow relation (`can_flow`).
 
+/// The monotonicity property of labels,
+/// formulated the usual way.
+
+val label_is_corrupt_later:
+  l:label ->
+  tr1:trace_ unit -> tr2:trace_ unit ->
+  Lemma
+  (requires
+    l.is_corrupt tr1 /\
+    tr1 <$ tr2
+  )
+  (ensures l.is_corrupt tr2)
+let label_is_corrupt_later l tr1 tr2 =
+  grows_induction_principle l.is_corrupt (fun tr ev ->
+    l.is_corrupt_later;
+    reveal_opaque (`%is_monotonic) is_monotonic
+  ) tr1 tr2
+
+/// Helper type and function to create labels.
+/// This takes care of the restricted arrow type,
+/// and the weird formulation of monotonicity in `is_corrupt_later`.
+
+noeq
+type label_constructor = {
+  is_corrupt: trace_ unit -> prop;
+  is_corrupt_later:
+    tr1:trace_ unit -> tr2:trace_ unit ->
+    Lemma
+    (requires is_corrupt tr1 /\ tr1 <$ tr2)
+    (ensures is_corrupt tr2)
+  ;
+}
+
+#push-options "--fuel 1"
+val mk_label: label_constructor -> label
+let mk_label l = {
+  is_corrupt = FStar.FunctionalExtensionality.on _ l.is_corrupt;
+  is_corrupt_later = (
+    reveal_opaque (`%is_monotonic) is_monotonic;
+    reveal_opaque (`%grows) (grows #unit);
+    norm_spec [zeta; delta_only [`%prefix]] (prefix #unit);
+    assert(forall (tr:trace_ unit) ev. tr <$ (Snoc tr ev));
+    FStar.Classical.forall_intro_2 (FStar.Classical.move_requires_2 l.is_corrupt_later)
+  );
+}
+#pop-options
+
 /// If the attacker knows a value with label `l`, then it must have done some corruptions in the trace.
 /// The corruption predicate express whether values with label `l` are still secure,
 /// with respect to corruption events in the trace.
@@ -62,7 +111,7 @@ val is_corrupt_later:
 let is_corrupt_later tr1 tr2 l =
   reveal_opaque (`%is_corrupt) (is_corrupt);
   trace_forget_labels_later tr1 tr2;
-  grows_induction_principle l.is_corrupt l.is_corrupt_later (trace_forget_labels tr1) (trace_forget_labels tr2)
+  label_is_corrupt_later l (trace_forget_labels tr1) (trace_forget_labels tr2)
 
 /// A label `l1` can flow to a label `l2` when `l2` will always be more secret than `l1` in the future,
 /// or more precisely, when in the future, a corruption of `l2` implies a corruption of `l1`.
@@ -73,53 +122,78 @@ let can_flow tr l1 l2 =
   forall tr_extended. tr <$ tr_extended ==>
     (is_corrupt tr_extended l2 ==> is_corrupt tr_extended l1)
 
+/// Extensionality theorems for labels
+
+val intro_label_equal:
+  l1:label -> l2:label ->
+  (tr:trace -> Lemma (l1 `can_flow tr` l2 /\ l2 `can_flow tr` l1)) ->
+  Lemma (l1 == l2)
+let intro_label_equal l1 l2 pf =
+  let open DY.Core.Label.Unknown in
+  reveal_opaque (`%can_flow) can_flow;
+  reveal_opaque (`%is_corrupt) is_corrupt;
+  introduce forall tr. l1.is_corrupt tr == l2.is_corrupt tr with (
+    pf (fmap_trace (forget_label unknown_label) tr);
+    // These two lines prove surjectivity of `trace_forget_labels`
+    // by showing that fmap_trace (forget_label public) is a right-inverse
+    // (we could replace `public` with anything)
+    fmap_trace_compose (forget_label unknown_label) (forget_label ()) (forget_label ()) tr;
+    fmap_trace_identity (forget_label ()) tr;
+    FStar.PropositionalExtensionality.apply (l1.is_corrupt tr) (l2.is_corrupt tr)
+  );
+  assert(l1.is_corrupt `FStar.FunctionalExtensionality.feq` l2.is_corrupt);
+  assert(l1.is_corrupt == l2.is_corrupt);
+  assert(l1.is_corrupt_later == l2.is_corrupt_later);
+  ()
+
+
 /// Functions to create labels.
 /// They are useful so that the label type can remain abstract to the user.
 
 [@@"opaque_to_smt"]
 val secret: label
-let secret = {
+let secret = mk_label {
   is_corrupt = (fun tr -> False);
   is_corrupt_later = (fun tr1 tr2 -> ());
 }
 
 [@@"opaque_to_smt"]
 val public: label
-let public = {
+let public = mk_label {
   is_corrupt = (fun tr -> True);
   is_corrupt_later = (fun tr1 tr2 -> ());
 }
 
 [@@"opaque_to_smt"]
 val meet: label -> label -> label
-let meet l1 l2 = {
+let meet l1 l2 = mk_label {
   is_corrupt = (fun tr -> l1.is_corrupt tr /\ l2.is_corrupt tr);
   is_corrupt_later = (fun tr1 tr2 ->
-    l1.is_corrupt_later tr1 tr2;
-    l2.is_corrupt_later tr1 tr2
+    label_is_corrupt_later l1 tr1 tr2;
+    label_is_corrupt_later l2 tr1 tr2
   );
 }
 
 [@@"opaque_to_smt"]
 val join: label -> label -> label
-let join l1 l2 = {
+let join l1 l2 = mk_label {
   is_corrupt = (fun tr -> l1.is_corrupt tr \/ l2.is_corrupt tr);
   is_corrupt_later = (fun tr1 tr2 ->
-    FStar.Classical.move_requires (l1.is_corrupt_later tr1) tr2;
-    FStar.Classical.move_requires (l2.is_corrupt_later tr1) tr2
+    FStar.Classical.move_requires_3 label_is_corrupt_later l1 tr1 tr2;
+    FStar.Classical.move_requires_3 label_is_corrupt_later l2 tr1 tr2
   );
 }
 
 [@@"opaque_to_smt"]
 val principal_label: principal -> label
-let principal_label prin = {
+let principal_label prin = mk_label {
   is_corrupt = (fun tr -> exists sess_id. was_corrupt tr prin sess_id);
   is_corrupt_later = (fun tr1 tr2 -> ());
 }
 
 [@@"opaque_to_smt"]
 val principal_state_label: principal -> state_id -> label
-let principal_state_label prin sess_id = {
+let principal_state_label prin sess_id = mk_label {
   is_corrupt = (fun tr -> was_corrupt tr prin sess_id);
   is_corrupt_later = (fun tr1 tr2 -> ());
 }
@@ -154,6 +228,7 @@ let extract_pre_label l =
     None
   )
 
+#push-options "--ifuel 1 --fuel 1"
 val principal_label_injective:
   p:principal ->
   Lemma (extract_pre_label (principal_label p) == Some (PreLabel_P p))
@@ -169,7 +244,9 @@ let principal_label_injective p =
   let tr_1: trace_ unit = (Snoc Nil (Corrupt p sess_id_1)) in
   assert_norm(event_at tr_1 0 (Corrupt p sess_id_1));
   assert(extract_pre_label_is_some l (p, sess_id_0))
+#pop-options
 
+#push-options "--ifuel 1 --fuel 1"
 val principal_state_label_injective:
   p:principal -> s:state_id ->
   Lemma (extract_pre_label (principal_state_label p s) == Some (PreLabel_S p s))
@@ -181,6 +258,7 @@ let principal_state_label_injective p s =
   let tr: trace_ unit = (Snoc Nil (Corrupt p s)) in
   assert_norm(event_at tr 0 (Corrupt p s));
   assert(extract_pre_label_is_some l (p, s))
+#pop-options
 
 /// `can_flow tr` is reflexive.
 
@@ -223,8 +301,9 @@ val secret_is_bottom:
   (ensures l `can_flow tr` secret)
   [SMTPat (l `can_flow tr` secret)]
 let secret_is_bottom tr l =
-  normalize_term_spec can_flow;
-  normalize_term_spec secret
+  reveal_opaque (`%can_flow) can_flow;
+  reveal_opaque (`%secret) secret;
+  reveal_opaque (`%is_corrupt) is_corrupt
 
 /// `secret` is the maximum of the label lattice.
 
@@ -234,8 +313,9 @@ val public_is_top:
   (ensures public `can_flow tr` l)
   [SMTPat (public `can_flow tr` l)]
 let public_is_top tr l =
-  normalize_term_spec can_flow;
-  normalize_term_spec public
+  reveal_opaque (`%can_flow) can_flow;
+  reveal_opaque (`%public) public;
+  reveal_opaque (`%is_corrupt) is_corrupt
 
 /// `meet` satisfy the lower bound property.
 
@@ -245,7 +325,7 @@ val meet_eq:
   (ensures meet y1 y2 `can_flow tr` x <==> (y1 `can_flow tr` x /\ y2 `can_flow tr` x))
   [SMTPat (meet y1 y2 `can_flow tr` x)] //Not sure about this
 let meet_eq tr x y1 y2 =
-  norm_spec [zeta; delta_only [`%is_corrupt]] (is_corrupt);
+  reveal_opaque (`%is_corrupt) (is_corrupt);
   reveal_opaque (`%can_flow) (can_flow);
   reveal_opaque (`%meet) (meet)
 
@@ -257,7 +337,7 @@ val join_eq:
   (ensures y `can_flow tr` join x1 x2 <==> (y `can_flow tr` x1 /\ y `can_flow tr` x2))
   [SMTPat (y `can_flow tr` join x1 x2)] //Not sure about this
 let join_eq tr x1 x2 y =
-  norm_spec [zeta; delta_only [`%is_corrupt]] (is_corrupt);
+  reveal_opaque (`%is_corrupt) (is_corrupt);
   reveal_opaque (`%can_flow) (can_flow);
   reveal_opaque (`%join) (join)
 
@@ -269,7 +349,7 @@ val flow_to_public_eq:
   (ensures l `can_flow tr` public <==> is_corrupt tr l)
   [SMTPat (l `can_flow tr` public)] //Not sure about this
 let flow_to_public_eq tr prin =
-  norm_spec [zeta; delta_only [`%is_corrupt]] (is_corrupt);
+  reveal_opaque (`%is_corrupt) (is_corrupt);
   reveal_opaque (`%can_flow) (can_flow);
   reveal_opaque (`%public) (public)
 
@@ -281,10 +361,10 @@ val principal_flow_to_principal_state:
   (ensures (principal_label prin) `can_flow tr` (principal_state_label prin sess_id))
   [SMTPat ((principal_label prin) `can_flow tr` (principal_state_label prin sess_id))]
 let principal_flow_to_principal_state tr prin sess_id =
-  norm_spec [zeta; delta_only [`%is_corrupt]] (is_corrupt);
-  normalize_term_spec can_flow;
-  normalize_term_spec principal_label;
-  normalize_term_spec principal_state_label
+  reveal_opaque (`%is_corrupt) is_corrupt;
+  reveal_opaque (`%can_flow) can_flow;
+  reveal_opaque (`%principal_label) principal_label;
+  reveal_opaque (`%principal_state_label) principal_state_label
 
 /// A `join` flows to `public` iff. one of its operands flows to `public`.
 /// This is a property specific to labels,
@@ -296,7 +376,7 @@ val join_flow_to_public_eq:
   (ensures (join x1 x2) `can_flow tr` public <==> x1 `can_flow tr` public \/ x2 `can_flow tr` public)
   [SMTPat ((join x1 x2) `can_flow tr` public)] //Not sure about this
 let join_flow_to_public_eq tr x1 x2 =
-  norm_spec [zeta; delta_only [`%is_corrupt]] (is_corrupt);
+  reveal_opaque (`%is_corrupt) is_corrupt;
   reveal_opaque (`%can_flow) (can_flow);
   reveal_opaque (`%join) (join);
   reveal_opaque (`%public) (public)
